defined fair beh

src/FairBeh.v
@@ -10,8 +10,8 @@ Set Implicit Arguments.
 
 Section OBS.
 
-  Variant event: Type :=
-    | event_syscall (fn: nat) (args: list nat) (retv: nat)
+  Variant obs: Type :=
+    | obs_syscall (fn: nat) (args: list nat) (retv: nat)
   .
 
 End OBS.
@@ -22,11 +22,11 @@ Module Tr.
   | spin
   | ub
   | nb
-  | cons (hd: event) (tl: t)
+  | cons (hd: obs) (tl: t)
   .
   Infix "##" := cons (at level 60, right associativity).
 
-  Fixpoint app {R} (pre: list event) (bh: @t R): t :=
+  Fixpoint app {R} (pre: list obs) (bh: @t R): t :=
     match pre with
     | [] => bh
     | hd :: tl => cons hd (app tl bh)
@@ -40,7 +40,7 @@ Module Tr.
   .
   Proof. reflexivity. Qed.
 
-  Definition prefix {R} (pre: list event) (bh: @t R): Prop :=
+  Definition prefix {R} (pre: list obs) (bh: @t R): Prop :=
     exists tl, <<PRE: app pre tl = bh>>
   .
 
@@ -85,51 +85,188 @@ Section EVENT.
   Variant eventE: Type -> Type :=
     | Choose (X: Type): eventE X
     | Fair (m: id -> Flag.t): eventE unit
-    | Syscall (fn: nat) (args: list nat) (retv: nat): eventE nat
+    | Observe (fn: nat) (args: list nat) (retv: nat): eventE nat
+    | Undefined: eventE void
   .
 
 End EVENT.
 
 
+
+(* Section STS. *)
+
+(*   Context {Ident: ID}. *)
+
+(*   Definition state {R} := itree eventE R. *)
+
+(*   Inductive step {R}: @state R -> option event -> state -> Prop := *)
+(*   | step_tau *)
+(*       itr *)
+(*     : *)
+(*     step (Tau itr) None itr *)
+(*   | step_choose *)
+(*       X ktr (x: X) *)
+(*     : *)
+(*     step (Vis (Choose X) ktr) None (ktr x) *)
+(*   | step_fair *)
+(*       m ktr *)
+(*     : *)
+(*     step (Vis (Fair m) ktr) None (ktr tt) *)
+(*   | step_syscall *)
+(*       fn args retv ktr *)
+(*     : *)
+(*     step (Vis (Syscall fn args retv) ktr) (Some (event_syscall fn args retv)) (ktr retv) *)
+(*   . *)
+
+(*   Lemma step_trigger_choose_iff X k itr e *)
+(*         (STEP: step (trigger (Choose X) >>= k) e itr) *)
+(*     : *)
+(*       exists x, *)
+(*         e = None /\ itr = k x. *)
+(*   Proof. *)
+(*     inv STEP. *)
+(*     { eapply f_equal with (f:=observe) in H0. ss. } *)
+(*     { eapply f_equal with (f:=observe) in H0. ss. *)
+(*       unfold trigger in H0. ss. cbn in H0. *)
+(*       dependent destruction H0. ired. et.  } *)
+(*     { eapply f_equal with (f:=observe) in H0. ss. } *)
+(*     { eapply f_equal with (f:=observe) in H0. ss. } *)
+(*   Qed. *)
+
+(*   Lemma step_trigger_take_iff X k itr e *)
+(*         (STEP: step (trigger (Take X) >>= k) e itr) *)
+(*     : *)
+(*       exists x, *)
+(*         e = None /\ itr = k x. *)
+(*   Proof. *)
+(*     inv STEP. *)
+(*     { eapply f_equal with (f:=observe) in H0. ss. } *)
+(*     { eapply f_equal with (f:=observe) in H0. ss. } *)
+(*     { eapply f_equal with (f:=observe) in H0. ss. *)
+(*       unfold trigger in H0. ss. cbn in H0. *)
+(*       dependent destruction H0. ired. et.  } *)
+(*     { eapply f_equal with (f:=observe) in H0. ss. } *)
+(*   Qed. *)
+
+(*   Lemma step_tau_iff itr0 itr1 e *)
+(*         (STEP: step (Tau itr0) e itr1) *)
+(*     : *)
+(*       e = None /\ itr0 = itr1. *)
+(*   Proof. *)
+(*     inv STEP. et. *)
+(*   Qed. *)
+
+(*   Lemma step_ret_iff rv itr e *)
+(*         (STEP: step (Ret rv) e itr) *)
+(*     : *)
+(*       False. *)
+(*   Proof. *)
+(*     inv STEP. *)
+(*   Qed. *)
+
+(*   Lemma step_trigger_syscall_iff fn args rvs k e itr *)
+(*         (STEP: step (trigger (Syscall fn args rvs) >>= k) e itr) *)
+(*     : *)
+(*       exists rv, itr = k rv /\ e = Some (event_sys fn args rv) *)
+(*                  /\ <<RV: rvs rv>> /\ <<SYS: syscall_sem (event_sys fn args rv)>>. *)
+(*   Proof. *)
+(*     inv STEP. *)
+(*     { eapply f_equal with (f:=observe) in H0. ss. } *)
+(*     { eapply f_equal with (f:=observe) in H0. ss. } *)
+(*     { eapply f_equal with (f:=observe) in H0. ss. } *)
+(*     { eapply f_equal with (f:=observe) in H0. ss. *)
+(*       unfold trigger in H0. ss. cbn in H0. *)
+(*       dependent destruction H0. ired. et. } *)
+(*   Qed. *)
+
+
+(*   Let itree_eta E R (itr0 itr1: itree E R) *)
+(*       (OBSERVE: observe itr0 = observe itr1) *)
+(*     : *)
+(*       itr0 = itr1. *)
+(*   Proof. *)
+(*     rewrite (itree_eta_ itr0). *)
+(*     rewrite (itree_eta_ itr1). *)
+(*     rewrite OBSERVE. auto. *)
+(*   Qed. *)
+
+(*   Lemma step_trigger_choose X k x *)
+(*     : *)
+(*       step (trigger (Choose X) >>= k) None (k x). *)
+(*   Proof. *)
+(*     unfold trigger. ss. *)
+(*     match goal with *)
+(*     | [ |- step ?itr _ _] => *)
+(*       replace itr with (Subevent.vis (Choose X) k) *)
+(*     end; ss. *)
+(*     { econs. } *)
+(*     { eapply itree_eta. ss. cbv. f_equal. *)
+(*       extensionality x0. eapply itree_eta. ss. } *)
+(*   Qed. *)
+
+(*   Lemma step_trigger_take X k x *)
+(*     : *)
+(*       step (trigger (Take X) >>= k) None (k x). *)
+(*   Proof. *)
+(*     unfold trigger. ss. *)
+(*     match goal with *)
+(*     | [ |- step ?itr _ _] => *)
+(*       replace itr with (Subevent.vis (Take X) k) *)
+(*     end; ss. *)
+(*     { econs. } *)
+(*     { eapply itree_eta. ss. cbv. f_equal. *)
+(*       extensionality x0. eapply itree_eta. ss. } *)
+(*   Qed. *)
+
+(*   Lemma step_trigger_syscall fn args (rvs: Any.t -> Prop) k rv *)
+(*         (RV: rvs rv) (SYS: syscall_sem (event_sys fn args rv)) *)
+(*     : *)
+(*       step (trigger (Syscall fn args rvs) >>= k) (Some (event_sys fn args rv)) (k rv). *)
+(*   Proof. *)
+(*     unfold trigger. ss. *)
+(*     match goal with *)
+(*     | [ |- step ?itr _ _] => *)
+(*       replace itr with (Subevent.vis (Syscall fn args rvs) k) *)
+(*     end; ss. *)
+(*     { econs; et. } *)
+(*     { eapply itree_eta. ss. cbv. f_equal. *)
+(*       extensionality x0. eapply itree_eta. ss. } *)
+(*   Qed. *)
+
+
+(* End STS. *)
+
+
+Section STS.
+
+  Context {Ident: ID}.
+
+  Definition state {R} := itree eventE R.
+  Definition imap := id -> nat.
+
+  Definition fair_update (m0 m1: imap) (f: id -> Flag.t) : Prop :=
+    forall j, match f j with
+         | Flag.fail => lt (m1 j) (m0 j)
+         | Flag.emp => le (m1 j) (m0 j)
+         | Flag.success => True
+         end.
+
+End STS.
+
+Module Beh.
+
+Definition t {R}: Type := @Tr.t R -> Prop.
+Definition improves {R} (src tgt: @t R): Prop := tgt <1= src.
+
 Section BEHAVES.
 
   Context {Ident: ID}.
 
-  Inductive terminate
-            (R: Type)
-    :
-    forall (itr: itree eventE R), Prop :=
-  | terminate_ret
-      r
-    :
-    terminate (Ret r)
-  | terminate_tau
-      itr
-      (TERM: terminate itr)
-    :
-    terminate (Tau itr)
-  | terminate_choose
-      X ktr x
-      (TERM: terminate (ktr x))
-    :
-    terminate (Vis (Choose X) ktr)
-  | terminate_fair
-      m ktr
-      (TERM: terminate (ktr tt))
-    :
-    terminate (Vis (Fair m) ktr)
-  | terminate_syscall
-      fn args retv ktr
-      (TERM: terminate (ktr retv))
-    :
-    terminate (Vis (Syscall fn args retv) ktr)
-  .
-
   Variant _diverge_index
-          (diverge_index: forall (R: Type) (idx: id -> nat) (itr: itree eventE R), Prop)
+          (diverge_index: forall (R: Type) (idx: imap) (itr: @state _ R), Prop)
           (R: Type)
     :
-    forall (idx: id -> nat) (itr: itree eventE R), Prop :=
+    forall (idx: imap) (itr: @state _ R), Prop :=
     | diverge_index_tau
         itr idx0 idx1
         (DIV: diverge_index _ idx1 itr)
@@ -143,18 +280,17 @@ Section BEHAVES.
       :
       _diverge_index diverge_index idx0 (Vis (Choose X) ktr)
     | diverge_index_fair
-        m ktr idx0 idx1
+        fmap ktr idx0 idx1
         (DIV: diverge_index _ idx1 (ktr tt))
-        (EMP: forall j (IDX: (m j) = Flag.emp), idx1 j <= idx0 j)
-        (FAIL: forall j (IDX: (m j) = Flag.fail), idx1 j < idx0 j)
+        (FAIR: fair_update idx0 idx1 fmap)
       :
-      _diverge_index diverge_index idx0 (Vis (Fair m) ktr)
-    | diverge_index_syscall
-        fn args retv ktr idx0 idx1
-        (DIV: diverge_index _ idx1 (ktr retv))
-        (IDX: forall i, idx1 i <= idx0 i)
-      :
-      _diverge_index diverge_index idx0 (Vis (Syscall fn args retv) ktr)
+      _diverge_index diverge_index idx0 (Vis (Fair fmap) ktr)
+    (* | diverge_index_syscall *)
+    (*     fn args retv ktr idx0 idx1 *)
+    (*     (DIV: diverge_index _ idx1 (ktr retv)) *)
+    (*     (IDX: forall i, idx1 i <= idx0 i) *)
+    (*   : *)
+    (*   _diverge_index diverge_index idx0 (Vis (Observe fn args retv) ktr) *)
   .
 
   Lemma diverge_index_mon: monotone3 _diverge_index.
@@ -163,298 +299,132 @@ Section BEHAVES.
     - econs 1; eauto.
     - econs 2; eauto.
     - econs 3; eauto.
-    - econs 4; eauto.
+    (* - econs 4; eauto. *)
   Qed.
 
-  Definition diverge_index: forall (R: Type) (idx: id -> nat) (itr: itree eventE R), Prop := paco3 _diverge_index bot3.
+  Definition diverge_index: forall (R: Type) (idx: imap) (itr: state), Prop := paco3 _diverge_index bot3.
 
-  Definition diverge (R: Type) (itr: itree eventE R): Prop :=
+  Hint Constructors _diverge_index.
+  Hint Unfold diverge_index.
+  Hint Resolve diverge_index_mon: paco.
+
+  Definition diverge (R: Type) (itr: @state _ R): Prop :=
     exists idx, diverge_index idx itr.
 
-End BEHAVES.
 
-
-
-Section STS.
-
-  Context {Ident: ID}.
-
-  Definition state {R} := itree eventE R.
-
-  Inductive step {R}: @state R -> option event -> state -> Prop :=
-  | step_tau
-      itr
-    :
-    step (Tau itr) None itr
-  | step_choose
-      X ktr (x: X)
-    :
-    step (Vis (Choose X) ktr) None (ktr x)
-  | step_fair
-      m ktr
-    :
-    step (Vis (Fair m) ktr) None (ktr tt)
-  | step_syscall
-      fn args retv ktr
-    :
-    step (Vis (Syscall fn args retv) ktr) (Some (event_syscall fn args retv)) (ktr retv)
-  .
-
-  Lemma step_trigger_choose_iff X k itr e
-        (STEP: step (trigger (Choose X) >>= k) e itr)
-    :
-      exists x,
-        e = None /\ itr = k x.
-  Proof.
-    inv STEP.
-    { eapply f_equal with (f:=observe) in H0. ss. }
-    { eapply f_equal with (f:=observe) in H0. ss.
-      unfold trigger in H0. ss. cbn in H0.
-      dependent destruction H0. ired. et.  }
-    { eapply f_equal with (f:=observe) in H0. ss. }
-    { eapply f_equal with (f:=observe) in H0. ss. }
-  Qed.
-
-  Lemma step_trigger_take_iff X k itr e
-        (STEP: step (trigger (Take X) >>= k) e itr)
-    :
-      exists x,
-        e = None /\ itr = k x.
-  Proof.
-    inv STEP.
-    { eapply f_equal with (f:=observe) in H0. ss. }
-    { eapply f_equal with (f:=observe) in H0. ss. }
-    { eapply f_equal with (f:=observe) in H0. ss.
-      unfold trigger in H0. ss. cbn in H0.
-      dependent destruction H0. ired. et.  }
-    { eapply f_equal with (f:=observe) in H0. ss. }
-  Qed.
-
-  Lemma step_tau_iff itr0 itr1 e
-        (STEP: step (Tau itr0) e itr1)
-    :
-      e = None /\ itr0 = itr1.
-  Proof.
-    inv STEP. et.
-  Qed.
-
-  Lemma step_ret_iff rv itr e
-        (STEP: step (Ret rv) e itr)
-    :
-      False.
-  Proof.
-    inv STEP.
-  Qed.
-
-  Lemma step_trigger_syscall_iff fn args rvs k e itr
-        (STEP: step (trigger (Syscall fn args rvs) >>= k) e itr)
-    :
-      exists rv, itr = k rv /\ e = Some (event_sys fn args rv)
-                 /\ <<RV: rvs rv>> /\ <<SYS: syscall_sem (event_sys fn args rv)>>.
-  Proof.
-    inv STEP.
-    { eapply f_equal with (f:=observe) in H0. ss. }
-    { eapply f_equal with (f:=observe) in H0. ss. }
-    { eapply f_equal with (f:=observe) in H0. ss. }
-    { eapply f_equal with (f:=observe) in H0. ss.
-      unfold trigger in H0. ss. cbn in H0.
-      dependent destruction H0. ired. et. }
-  Qed.
-
-
-  Let itree_eta E R (itr0 itr1: itree E R)
-      (OBSERVE: observe itr0 = observe itr1)
-    :
-      itr0 = itr1.
-  Proof.
-    rewrite (itree_eta_ itr0).
-    rewrite (itree_eta_ itr1).
-    rewrite OBSERVE. auto.
-  Qed.
-
-  Lemma step_trigger_choose X k x
-    :
-      step (trigger (Choose X) >>= k) None (k x).
-  Proof.
-    unfold trigger. ss.
-    match goal with
-    | [ |- step ?itr _ _] =>
-      replace itr with (Subevent.vis (Choose X) k)
-    end; ss.
-    { econs. }
-    { eapply itree_eta. ss. cbv. f_equal.
-      extensionality x0. eapply itree_eta. ss. }
-  Qed.
-
-  Lemma step_trigger_take X k x
-    :
-      step (trigger (Take X) >>= k) None (k x).
-  Proof.
-    unfold trigger. ss.
-    match goal with
-    | [ |- step ?itr _ _] =>
-      replace itr with (Subevent.vis (Take X) k)
-    end; ss.
-    { econs. }
-    { eapply itree_eta. ss. cbv. f_equal.
-      extensionality x0. eapply itree_eta. ss. }
-  Qed.
-
-  Lemma step_trigger_syscall fn args (rvs: Any.t -> Prop) k rv
-        (RV: rvs rv) (SYS: syscall_sem (event_sys fn args rv))
-    :
-      step (trigger (Syscall fn args rvs) >>= k) (Some (event_sys fn args rv)) (k rv).
-  Proof.
-    unfold trigger. ss.
-    match goal with
-    | [ |- step ?itr _ _] =>
-      replace itr with (Subevent.vis (Syscall fn args rvs) k)
-    end; ss.
-    { econs; et. }
-    { eapply itree_eta. ss. cbv. f_equal.
-      extensionality x0. eapply itree_eta. ss. }
-  Qed.
-
-
-End STS.
-
-
-
-
-Module Beh.
-
-Definition t: Type := Tr.t -> Prop.
-Definition improves (src tgt: t): Prop := tgt <1= src.
-
-Section BEHAVES.
-
-  Definition union (st0: state) (P: (option event) -> state -> Prop) :=
-    exists ev st1, (<<STEP: L.(step) st0 ev st1>>) /\ (<<UNION: P ev st1>>).
+  (* Definition union {R} (st0: @state R) (P: (option obs) -> (@state R) -> Prop) := *)
+  (*   exists ev st1, (<<STEP: L.(step) st0 ev st1>>) /\ (<<UNION: P ev st1>>). *)
   (* Definition inter (st0: L.(state)) (P: (option event) -> L.(state) -> Prop) := *)
   (*   forall ev st1 (STEP: L.(step) st0 ev st1), <<INTER: P ev st1>>. *)
 
-  Inductive _state_spin (state_spin: L.(state) -> Prop)
-            (st0: L.(state)): Prop :=
-  | state_spin_angelic
-      (SRT: L.(state_sort) st0 = angelic)
-      (STEP: forall ev st1 (STEP: L.(step) st0 ev st1), <<TL: state_spin st1>>)
-  | state_spin_demonic
-      (SRT: L.(state_sort) st0 = demonic)
-      (STEP: exists ev st1 (STEP: L.(step) st0 ev st1), <<TL: state_spin st1>>)
+
+  Inductive _of_state
+            (of_state: forall (R: Type), imap -> (@state _ R) -> (@Tr.t R) -> Prop)
+            (R: Type)
+    :
+    imap -> (@state _ R) -> Tr.t -> Prop :=
+  | done
+      imap0 retv
+    :
+    _of_state of_state imap0 (Ret retv) (Tr.done retv)
+  | spin
+      imap0 st0
+      (SPIN: diverge_index imap0 st0)
+    :
+    _of_state of_state imap0 st0 (Tr.spin)
+  | nb
+      imap0 st0
+    :
+    _of_state of_state imap0 st0 (Tr.nb)
+  | obs
+      imap0 imap1 fn args rv ktr tl
+      (IMAP: forall j, le (imap1 j) (imap0 j))
+      (TL: of_state _ imap1 (ktr rv) tl)
+    :
+    _of_state of_state imap0 (Vis (Observe fn args rv) ktr) (Tr.cons (obs_syscall fn args rv) tl)
+
+  | tau
+      imap0 imap1 itr tr
+      (IMAP: forall j, le (imap1 j) (imap0 j))
+      (STEP: _of_state of_state imap1 itr tr)
+    :
+    _of_state of_state imap0 (Tau itr) tr
+  | choose
+      imap0 imap1 X ktr x tr
+      (IMAP: forall j, le (imap1 j) (imap0 j))
+      (STEP: _of_state of_state imap1 (ktr x) tr)
+    :
+    _of_state of_state imap0 (Vis (Choose X) ktr) tr
+  | fair
+      imap0 imap1 fmap ktr tr
+      (FMAP: fair_update imap0 imap1 fmap)
+      (STEP: _of_state of_state imap1 (ktr tt) tr)
+      (* (STEP: union st0 (fun e st1 => (<<HD: e = None>>) /\ (<<TL: _of_state of_state st1 evs>>))) *)
+    :
+    _of_state of_state imap0 (Vis (Fair fmap) ktr) tr
+  (* | sb_angelic *)
+  (*     st0 *)
+  (*     evs *)
+  (*     (SRT: L.(state_sort) st0 = angelic) *)
+  (*     (STEP: inter st0 (fun e st1 => (<<HD: e = None>>) /\ (<<TL: _of_state of_state st1 evs>>))) *)
+  (*   : *)
+  (*   _of_state of_state st0 evs *)
   .
 
-  Definition state_spin: _ -> Prop := paco1 _state_spin bot1.
+  Definition of_state: forall (R: Type),  imap -> state -> Tr.t -> Prop := paco4 _of_state bot4.
 
-  Lemma state_spin_mon: monotone1 _state_spin.
-  Proof.
-    ii. inv IN; try (by econs; eauto).
-    - econs 1; et. ii. exploit STEP; et.
-    - des. econs 2; et. esplits; et.
-  Qed.
-
-  Hint Constructors _state_spin.
-  Hint Unfold state_spin.
-  Hint Resolve state_spin_mon: paco.
-
-
-
-  Inductive _of_state (of_state: L.(state) -> Tr.t -> Prop): L.(state) -> Tr.t -> Prop :=
-  | sb_final
-      st0 retv
-      (FINAL: L.(state_sort) st0 = final retv)
-    :
-    _of_state of_state st0 (Tr.done retv)
-  | sb_spin
-      st0
-      (SPIN: state_spin st0)
-    :
-    _of_state of_state st0 (Tr.spin)
-  | sb_nb
-      st0
-    :
-    _of_state of_state st0 (Tr.nb)
-  | sb_vis
-      st0 st1 ev evs
-      (SRT: L.(state_sort) st0 = vis)
-      (STEP: _.(step) st0 (Some ev) st1)
-      (TL: of_state st1 evs)
-    :
-    _of_state of_state st0 (Tr.cons ev evs)
-  | sb_demonic
-      st0
-      evs
-      (SRT: L.(state_sort) st0 = demonic)
-      (STEP: union st0 (fun e st1 => (<<HD: e = None>>) /\ (<<TL: _of_state of_state st1 evs>>)))
-    :
-    _of_state of_state st0 evs
-  | sb_angelic
-      st0
-      evs
-      (SRT: L.(state_sort) st0 = angelic)
-      (STEP: inter st0 (fun e st1 => (<<HD: e = None>>) /\ (<<TL: _of_state of_state st1 evs>>)))
-    :
-    _of_state of_state st0 evs
-  .
-
-  Definition of_state: _ -> _ -> Prop := paco2 _of_state bot2.
-
-  Theorem of_state_ind :
-    forall (r P: _ -> _ -> Prop),
-      (forall st0 retv, state_sort L st0 = final retv -> P st0 (Tr.done retv)) ->
-      (forall st0, state_spin st0 -> P st0 Tr.spin) ->
-      (forall st0, P st0 Tr.nb) ->
-
-      (forall st0 st1 ev evs
-         (SRT: state_sort L st0 = vis)
-         (STEP: _.(step) st0 (Some ev) st1)
-         (TL: r st1 evs)
+  Theorem of_state_ind:
+    forall (r: forall (R: Type), imap -> state -> Tr.t -> Prop) R (P: imap -> state -> Tr.t -> Prop),
+      (forall imap0 retv, P imap0 (Ret retv) (Tr.done retv)) ->
+      (forall imap0 st0, diverge_index imap0 st0 -> P imap0 st0 Tr.spin) ->
+      (forall imap0 st0, P imap0 st0 Tr.nb) ->
+      (forall imap0 imap1 fn args rv ktr tl
+         (IMAP: forall j, le (imap1 j) (imap0 j))
+         (TL: r _ imap1 (ktr rv) tl)
         ,
-          P st0 (Tr.cons ev evs)) ->
-      (forall st0 evs
-         (SRT: state_sort L st0 = demonic)
-         (STEP: union st0
-                      (fun e st1 =>
-                         <<HD: e = None >> /\ <<TL: _of_state r st1 evs >> /\ <<IH: P st1 evs>>)), P st0 evs) ->
-      (forall st0 evs
-         (* (IH: forall st1 (STEP: L.(step) st0 None st1), P st1 evs) *)
-         (SRT: state_sort L st0 = angelic)
-         (STEP: inter st0
-                      (fun e st1 => <<HD: e = None >> /\ <<TL: _of_state r st1 evs >> /\ <<IH: P st1 evs>>)),
-          P st0 evs) ->
-      forall s t, _of_state r s t -> P s t.
+          P imap0 (Vis (Observe fn args rv) ktr) (Tr.cons (obs_syscall fn args rv) tl)) ->
+      (forall imap0 imap1 itr tr
+         (IMAP: forall j, le (imap1 j) (imap0 j))
+         (STEP: _of_state r imap1 itr tr)
+         (IH: P imap1 itr tr)
+        ,
+          P imap0 (Tau itr) tr) ->
+      (forall imap0 imap1 X ktr x tr
+         (IMAP: forall j, le (imap1 j) (imap0 j))
+         (STEP: _of_state r imap1 (ktr x) tr)
+         (IH: P imap1 (ktr x) tr)
+        ,
+          P imap0 (Vis (Choose X) ktr) tr) ->
+      (forall imap0 imap1 fmap ktr tr
+         (FAIR: fair_update imap0 imap1 fmap)
+         (STEP: _of_state r imap1 (ktr tt) tr)
+         (IH: P imap1 (ktr tt) tr)
+        ,
+          P imap0 (Vis (Fair fmap) ktr) tr) ->
+      forall i s t, @_of_state r R i s t -> P i s t.
   Proof.
-    (* fix IH 11. i. *)
-    (* inv H5; eauto. *)
-    (* - eapply H3; eauto. rr in STEP. des; clarify. *)
-    (*   + esplits; eauto. rr. esplits; eauto. left. esplits; eauto. eapply IH; eauto. Guarded. *)
-    (*   + esplits; eauto. rr. esplits; eauto. right. esplits; eauto. *)
-    (* - eapply H4; eauto. ii. exploit STEP; eauto. i; des; clarify. *)
-    (*   + esplits; eauto. left. esplits; eauto. eapply IH; eauto. *)
-    (*   + esplits; eauto. right. esplits; eauto. *)
-    fix IH 11. i.
-    inv H5; eauto.
-    - eapply H3; eauto. rr in STEP. des; clarify. esplits; eauto. rr. esplits; eauto. eapply IH; eauto.
-    - eapply H4; eauto. ii. exploit STEP; eauto. i; des; clarify. esplits; eauto. eapply IH; eauto.
+    fix IH 14. i.
+    inv H6; eauto.
+    - eapply H3; eauto. eapply IH; eauto.
+    - eapply H4; eauto. eapply IH; eauto.
+    - eapply H5; eauto. eapply IH; eauto.
   Qed.
 
-  Lemma of_state_mon: monotone2 _of_state.
+  Lemma of_state_mon: monotone4 _of_state.
   Proof.
     ii. induction IN using of_state_ind; eauto.
-    - econs 1; et.
-    - econs 2; et.
-    - econs 3; et.
-    - econs 4; et.
-    - econs 5; et. rr in STEP. des; clarify. rr. esplits; et.
-    - econs 6; et. ii. exploit STEP; eauto. i; des; clarify.
+    - econs 1; eauto.
+    - econs 2; eauto.
+    - econs 3; eauto.
+    - econs 4; eauto.
+    - econs 5; eauto.
+    - econs 6; eauto.
+    - econs 7; eauto.
   Qed.
 
   Hint Constructors _of_state.
   Hint Unfold of_state.
   Hint Resolve of_state_mon: paco.
-
-  Definition of_program: Tr.t -> Prop := of_state L.(initial_state).
-
-
 
 
   (**********************************************************)
